

## Solutions

### Problem 1: Stock price over two days

#### 1. Outcomes, events, and probabilities

Let  $U$  denote “up by 2” and  $D$  denote “down by 2” on a given day. Over two days, the possible paths and resulting prices  $S_2$  are:

Outcome	Price	$\mathbb{P}(\text{Outcome})$
$UU$	$10 + 2 + 2 = 14$	$\frac{1}{2} \cdot \frac{1}{2} = \frac{1}{4}$
$UD$	$10 + 2 - 2 = 10$	$\frac{1}{2} \cdot \frac{1}{2} = \frac{1}{4}$
$DU$	$10 - 2 + 2 = 10$	$\frac{1}{2} \cdot \frac{1}{2} = \frac{1}{4}$
$DD$	$10 - 2 - 2 = 6$	$\frac{1}{2} \cdot \frac{1}{2} = \frac{1}{4}$

Thus the probability mass function of  $S_2$  is:

$$\mathbb{P}(S_2 = 6) = \frac{1}{4}, \quad \mathbb{P}(S_2 = 10) = \frac{1}{2}, \quad \mathbb{P}(S_2 = 14) = \frac{1}{4}.$$

#### 2. CDF of $S_2$

Define  $F(x) = \mathbb{P}(S_2 \leq x)$ . Then

$$F(x) = \begin{cases} 0, & x < 6, \\ \frac{1}{4}, & 6 \leq x < 10, \\ \frac{3}{4}, & 10 \leq x < 14, \\ 1, & x \geq 14. \end{cases}$$

This is a step function with jumps at  $x = 6, 10, 14$ .

#### 3. Expectation and variance of $S_2$

$$\mathbb{E}[S_2] = 6 \cdot \frac{1}{4} + 10 \cdot \frac{1}{2} + 14 \cdot \frac{1}{4} = \frac{6 + 20 + 14}{4} = \frac{40}{4} = 10.$$

Using the fact that  $\mathbb{V}[X] = \mathbb{E}[X^2] - (\mathbb{E}[X])^2$ ,

$$\mathbb{E}[S_2^2] = 6^2 \cdot \frac{1}{4} + 10^2 \cdot \frac{1}{2} + 14^2 \cdot \frac{1}{4} = \frac{36}{4} + \frac{100}{2} + \frac{196}{4} = 9 + 50 + 49 = 108.$$

$$\text{Var}(S_2) = \mathbb{E}[S_2^2] - (\mathbb{E}[S_2])^2 = 108 - 10^2 = 108 - 100 = 8.$$

#### 4. Contract payoff as a random variable and its expectation

At the end of day two you may buy one share at a fixed price of 11. If the market price is  $S_2$ , your profit (payoff) is

$$X = \max\{0, S_2 - 11\}.$$

This is a random variable: it assigns a real number (profit or loss) to each outcome of  $S_2$ .

From the distribution:

$S_2$	$\max\{0, S_2 - 11\}$	$\mathbb{P}$
6	0	$\frac{1}{4}$
10	0	$\frac{1}{2}$
14	3	$\frac{1}{4}$

Thus,

$$\mathbb{E}[X] = \frac{1}{4}0 + \frac{1}{2}0 + \frac{1}{4}3 = \frac{3}{4}.$$

### Problem 1: Hospital capacity

Let  $T$  be the length of stay (in days) for a patient who is admitted. Conditional on admission,  $T \sim \text{Unif}(0, 30)$  with CDF

$$F_T(t) = \begin{cases} 0, & t < 0, \\ \frac{t}{30}, & 0 \leq t \leq 30, \\ 1, & t > 30. \end{cases}$$

Let  $X$  be the length of stay for a random ER arrival, with  $X = 0$  if not admitted.

#### (a) Overall distribution function

With probability  $4/5$  the patient is not admitted and  $X = 0$ . With probability  $1/5$  they are admitted and  $X = T$ .

For  $t < 0$ ,

$$F_X(t) = \mathbb{P}(X \leq t) = 0.$$

For  $0 \leq t \leq 30$ ,

$$F_X(t) = \mathbb{P}(X = 0) + \mathbb{P}(\text{admitted and } T \leq t) = \frac{4}{5} + \frac{1}{5}\mathbb{P}(T \leq t) = \frac{4}{5} + \frac{1}{5} \cdot \frac{t}{30} = \frac{4}{5} + \frac{t}{150}.$$

For  $t > 30$ ,

$$F_X(t) = 1.$$

So

$$F_X(t) = \begin{cases} 0, & t < 0, \\ \frac{4}{5} + \frac{t}{150}, & 0 \leq t \leq 30, \\ 1, & t > 30. \end{cases}$$

There is a jump of size  $4/5$  at  $t = 0$  (point mass at 0), and a linear increase from  $4/5$  to 1 on  $[0, 30]$ .

(b) **Given admitted: expectation and variance**

If admitted,  $T \sim \text{Unif}(0, 30)$ . For  $U \sim \text{Unif}(a, b)$ ,

$$\mathbb{E}[U] = \frac{a+b}{2}, \quad \text{Var}(U) = \frac{(b-a)^2}{12}.$$

Here  $a = 0$ ,  $b = 30$ , so

$$\mathbb{E}[T] = \frac{0+30}{2} = 15, \quad \text{Var}(T) = \frac{30^2}{12} = \frac{900}{12} = 75.$$

(c) **Expected stay for a random ER arrival**

Let  $A$  denote the event “admitted”. Then

$$\mathbb{E}[X] = \mathbb{E}[X \mid A]\mathbb{P}(A) + \mathbb{E}[X \mid A^c]\mathbb{P}(A^c).$$

We have  $\mathbb{P}(A) = \frac{1}{5}$ ,  $\mathbb{P}(A^c) = \frac{4}{5}$ ,

$$\mathbb{E}[X \mid A] = \mathbb{E}[T] = 15, \quad \mathbb{E}[X \mid A^c] = 0.$$

Thus

$$\mathbb{E}[X] = 15 \cdot \frac{1}{5} + 0 \cdot \frac{4}{5} = 3 \text{ days}.$$

(d) **Expected number admitted and expected total bed-days**

If  $n$  patients arrive tomorrow and each is admitted independently with probability  $1/5$ , then the number admitted

$$N \sim \text{Binomial}\left(n, \frac{1}{5}\right),$$

so

$$\mathbb{E}[N] = n \cdot \frac{1}{5} = \frac{n}{5}.$$

For total bed-days, each ER arrival contributes an expected  $\mathbb{E}[X] = 3$  days. Let  $X_i$  be the stay length for patient  $i$ . Then the total bed-days is  $S = \sum_{i=1}^n X_i$ , and

$$\mathbb{E}[S] = \sum_{i=1}^n \mathbb{E}[X_i] = n \cdot 3 = 3n.$$

## Problem 2: Softmax choice over three options

We have three options  $a, b, c$  with values  $v_a > v_b > v_c$ , and probability mass function

$$\mathbb{P}[a] = \frac{e^{v_a/\sigma}}{Z}, \quad \mathbb{P}[b] = \frac{e^{v_b/\sigma}}{Z}, \quad \mathbb{P}[c] = \frac{e^{v_c/\sigma}}{Z},$$

where

$$Z = e^{v_a/\sigma} + e^{v_b/\sigma} + e^{v_c/\sigma}, \quad \sigma > 0.$$

(a) **Axioms of probability**

Each probability is nonnegative because exponentials are positive and  $Z > 0$ :

$$e^{v_i/\sigma} > 0, \quad Z = \sum_i e^{v_i/\sigma} > 0 \Rightarrow \mathbb{P}[i] = \frac{e^{v_i/\sigma}}{Z} \geq 0.$$

The probabilities sum to 1:

$$\mathbb{P}[a] + \mathbb{P}[b] + \mathbb{P}[c] = \frac{e^{v_a/\sigma} + e^{v_b/\sigma} + e^{v_c/\sigma}}{Z} = \frac{Z}{Z} = 1.$$

(b) **Independence of irrelevant alternatives (ratio  $p[a]/p[b]$ )**

With all three options present,

$$\frac{\mathbb{P}[a]}{\mathbb{P}[b]} = \frac{\frac{e^{v_a/\sigma}}{Z}}{\frac{e^{v_b/\sigma}}{Z}} = \frac{e^{v_a/\sigma}}{e^{v_b/\sigma}} = e^{(v_a - v_b)/\sigma}.$$

If we remove option  $c$ , the updated probabilities are

$$\mathbb{P}'[a] = \frac{e^{v_a/\sigma}}{e^{v_a/\sigma} + e^{v_b/\sigma}}, \quad \mathbb{P}'[b] = \frac{e^{v_b/\sigma}}{e^{v_a/\sigma} + e^{v_b/\sigma}}.$$

Then

$$\frac{\mathbb{P}'[a]}{\mathbb{P}'[b]} = \frac{\frac{e^{v_a/\sigma}}{e^{v_a/\sigma} + e^{v_b/\sigma}}}{\frac{e^{v_b/\sigma}}{e^{v_a/\sigma} + e^{v_b/\sigma}}} = \frac{e^{v_a/\sigma}}{e^{v_b/\sigma}} = e^{(v_a - v_b)/\sigma}.$$

Thus

$$\frac{\mathbb{P}[a]}{\mathbb{P}[b]} = \frac{\mathbb{P}'[a]}{\mathbb{P}'[b]},$$

so the ratio of  $a$  to  $b$  does not depend on whether  $c$  is present.

(c) **Effect of increasing  $v_a$**

Let  $v_b, v_c, \sigma$  be fixed and consider  $v_a$  as a variable.

First, note

$$\mathbb{P}[a] = \frac{e^{v_a/\sigma}}{e^{v_a/\sigma} + e^{v_b/\sigma} + e^{v_c/\sigma}}.$$

Differentiate with respect to  $v_a$ :

$$\frac{\partial \mathbb{P}[a]}{\partial v_a} = \frac{\frac{1}{\sigma} e^{v_a/\sigma} (e^{v_a/\sigma} + e^{v_b/\sigma} + e^{v_c/\sigma}) - e^{v_a/\sigma} \cdot \frac{1}{\sigma} e^{v_a/\sigma}}{(e^{v_a/\sigma} + e^{v_b/\sigma} + e^{v_c/\sigma})^2}.$$

This simplifies to

$$\frac{\partial \mathbb{P}[a]}{\partial v_a} = \frac{\frac{1}{\sigma} e^{v_a/\sigma} (e^{v_b/\sigma} + e^{v_c/\sigma})}{(e^{v_a/\sigma} + e^{v_b/\sigma} + e^{v_c/\sigma})^2} > 0,$$

because all terms are positive. Thus  $\mathbb{P}[a]$  increases as  $v_a$  increases.

For  $b$  and  $c$ , note that  $\mathbb{P}[a] + \mathbb{P}[b] + \mathbb{P}[c] = 1$ , so

$$\frac{\partial \mathbb{P}[b]}{\partial v_a} + \frac{\partial \mathbb{P}[c]}{\partial v_a} = -\frac{\partial \mathbb{P}[a]}{\partial v_a} < 0.$$

By symmetry, direct calculation also shows

$$\frac{\partial \mathbb{P}[b]}{\partial v_a} < 0, \quad \frac{\partial \mathbb{P}[c]}{\partial v_a} < 0.$$

Hence as  $v_a$  increases,  $\mathbb{P}[a]$  goes up, while  $\mathbb{P}[b]$  and  $\mathbb{P}[c]$  go down.

(d) **Limits as  $\sigma \rightarrow \infty$  and  $\sigma \rightarrow 0$**

As  $\sigma \rightarrow \infty$ , for each fixed  $v_i$ ,

$$\frac{v_i}{\sigma} \rightarrow 0 \quad \Rightarrow \quad e^{v_i/\sigma} \rightarrow e^0 = 1.$$

Therefore,

$$\mathbb{P}[a] \rightarrow \frac{1}{1+1+1} = \frac{1}{3}, \quad \mathbb{P}[b] \rightarrow \frac{1}{3}, \quad \mathbb{P}[c] \rightarrow \frac{1}{3},$$

so the probabilities become uniform.

As  $\sigma \rightarrow 0^+$ , divide numerator and denominator of  $\mathbb{P}[a]$  by  $e^{v_a/\sigma}$ :

$$\mathbb{P}[a] = \frac{1}{1 + e^{(v_b - v_a)/\sigma} + e^{(v_c - v_a)/\sigma}}.$$

Since  $v_b < v_a$  and  $v_c < v_a$ , we have  $v_b - v_a < 0$  and  $v_c - v_a < 0$ , so for  $\sigma \rightarrow 0^+$ ,

$$e^{(v_b - v_a)/\sigma} \rightarrow 0, \quad e^{(v_c - v_a)/\sigma} \rightarrow 0.$$

Thus

$$\lim_{\sigma \rightarrow 0^+} \mathbb{P}[a] = \frac{1}{1+0+0} = 1, \quad \lim_{\sigma \rightarrow 0^+} \mathbb{P}[b] = 0, \quad \lim_{\sigma \rightarrow 0^+} \mathbb{P}[c] = 0.$$

So in the limit  $\sigma \rightarrow 0^+$ , softmax selects the option with the highest value (here  $a$ ) with probability 1; this is the “hard max” limit.

## Problem 2: Weather Markov chain

States: Clear (C) and Rainy (R). Transition matrix (column-stochastic) is

$$P = \begin{pmatrix} 0.6 & 0.4 \\ 0.4 & 0.6 \end{pmatrix},$$

where  $p_{i \leftarrow j}$  is the probability of going from state  $j$  to state  $i$ .

Let the forecast vector be a column vector

$$v = \begin{pmatrix} \mathbb{P}(\text{Clear}) \\ \mathbb{P}(\text{Rainy}) \end{pmatrix}.$$

The update rule is  $v_{\text{next}} = Pv_{\text{current}}$ .

Assume today is clear, so

$$v_0 = \begin{pmatrix} 1 \\ 0 \end{pmatrix}.$$

### (a) Forecast for tomorrow

$$v_1 = Pv_0 = \begin{pmatrix} 0.6 & 0.4 \\ 0.4 & 0.6 \end{pmatrix} \begin{pmatrix} 1 \\ 0 \end{pmatrix} = \begin{pmatrix} 0.6 \\ 0.4 \end{pmatrix}.$$

So tomorrow: 60% chance Clear, 40% chance Rainy.

### (b) Forecast for the day after tomorrow

$$v_2 = Pv_1 = P^2v_0.$$

First compute  $P^2$ :

$$P^2 = \begin{pmatrix} 0.6 & 0.4 \\ 0.4 & 0.6 \end{pmatrix} \begin{pmatrix} 0.6 & 0.4 \\ 0.4 & 0.6 \end{pmatrix} = \begin{pmatrix} 0.36 + 0.16 & 0.24 + 0.24 \\ 0.24 + 0.24 & 0.16 + 0.36 \end{pmatrix} = \begin{pmatrix} 0.52 & 0.48 \\ 0.48 & 0.52 \end{pmatrix}.$$

Then

$$v_2 = P^2v_0 = \begin{pmatrix} 0.52 \\ 0.48 \end{pmatrix}.$$

So on the second day: 52% Clear, 48% Rainy.

### (c) Forecast for the third day

$$v_3 = Pv_2 = \begin{pmatrix} 0.6 & 0.4 \\ 0.4 & 0.6 \end{pmatrix} \begin{pmatrix} 0.52 \\ 0.48 \end{pmatrix} = \begin{pmatrix} 0.6 \cdot 0.52 + 0.4 \cdot 0.48 \\ 0.4 \cdot 0.52 + 0.6 \cdot 0.48 \end{pmatrix} = \begin{pmatrix} 0.504 \\ 0.496 \end{pmatrix}.$$

So on the third day: 50.4% Clear, 49.6% Rainy.

(d) **Show  $(0.5, 0.5)$  is stationary**

Let

$$v^* = \begin{pmatrix} 0.5 \\ 0.5 \end{pmatrix}.$$

Then

$$Pv^* = \begin{pmatrix} 0.6 & 0.4 \\ 0.4 & 0.6 \end{pmatrix} \begin{pmatrix} 0.5 \\ 0.5 \end{pmatrix} = \begin{pmatrix} 0.6 \cdot 0.5 + 0.4 \cdot 0.5 \\ 0.4 \cdot 0.5 + 0.6 \cdot 0.5 \end{pmatrix} = \begin{pmatrix} 0.5 \\ 0.5 \end{pmatrix} = v^*.$$

Thus if the current forecast is  $(0.5, 0.5)$ , the next forecast remains  $(0.5, 0.5)$ ; this is a stationary distribution.

### Problem 3: Poisson model and MLE

We have  $X \sim \text{Poisson}(\lambda)$  with

$$\mathbb{P}[X = k] = \frac{\lambda^k e^{-\lambda}}{k!}, \quad k = 0, 1, 2, \dots, \lambda > 0.$$

(a) **Poisson pmf obeys probability axioms**

Non-negativity: for all  $k$ ,  $\lambda^k \geq 0$ ,  $e^{-\lambda} > 0$ ,  $k! > 0$ , so

$$\mathbb{P}[X = k] = \frac{\lambda^k e^{-\lambda}}{k!} \geq 0.$$

Sum to 1:

$$\sum_{k=0}^{\infty} \mathbb{P}[X = k] = \sum_{k=0}^{\infty} \frac{\lambda^k e^{-\lambda}}{k!} = e^{-\lambda} \sum_{k=0}^{\infty} \frac{\lambda^k}{k!} = e^{-\lambda} e^{\lambda} = 1,$$

using the given hint.

(b) **Likelihood for sample  $x_1 = 1, x_2 = 2, x_3 = 3$**

Assuming  $X_1, X_2, X_3$  are independent  $\text{Poisson}(\lambda)$ , the likelihood is

$$L(\lambda) = \prod_{i=1}^3 \mathbb{P}[X_i = x_i] = \prod_{i=1}^3 \frac{\lambda^{x_i} e^{-\lambda}}{x_i!}.$$

With  $x_1 = 1, x_2 = 2, x_3 = 3$ ,

$$L(\lambda) = \frac{\lambda^1 e^{-\lambda}}{1!} \cdot \frac{\lambda^2 e^{-\lambda}}{2!} \cdot \frac{\lambda^3 e^{-\lambda}}{3!} = \frac{\lambda^6 e^{-3\lambda}}{1! 2! 3!}.$$

(c) **Maximum likelihood estimator**

Log-likelihood:

$$\ell(\lambda) = \log L(\lambda) = 6 \log \lambda - 3\lambda - \log(1! 2! 3!).$$

Differentiate and set to zero:

$$\ell'(\lambda) = \frac{6}{\lambda} - 3 = 0 \quad \Rightarrow \quad \frac{6}{\lambda} = 3 \quad \Rightarrow \quad \hat{\lambda} = 2.$$

(d) **Probability  $X \leq 2$  under fitted model**

Under the fitted model,  $X \sim \text{Poisson}(2)$ . Then

$$\mathbb{P}[X \leq 2] = \mathbb{P}[X = 0] + \mathbb{P}[X = 1] + \mathbb{P}[X = 2] = \sum_{k=0}^2 \frac{2^k e^{-2}}{k!}.$$

Compute:

$$\mathbb{P}[X \leq 2] = e^{-2} \left( \frac{2^0}{0!} + \frac{2^1}{1!} + \frac{2^2}{2!} \right) = e^{-2}(1 + 2 + 2) = 5e^{-2}.$$

### Problem 3: Categorical model and MLE

We observe 4 independent draws from a categorical distribution over labels  $\{a, b, c\}$ :

$a$  once,    $b$  twice,    $c$  once.

Let the probabilities be  $p_a, p_b, p_c$ .

(a) **Axioms of probability**

For a valid pmf over  $\{a, b, c\}$ , the probabilities must satisfy:

$$p_a \geq 0, \quad p_b \geq 0, \quad p_c \geq 0, \quad p_a + p_b + p_c = 1.$$

(b) **Likelihood for the data**

Let the counts be  $n_a = 1, n_b = 2, n_c = 1$ , with total  $n = 4$ .

Up to a combinatorial constant, the likelihood is

$$L(p_a, p_b, p_c) = p_a^{n_a} p_b^{n_b} p_c^{n_c} = p_a^1 p_b^2 p_c^1.$$

(If we include the multinomial coefficient,  $L$  is  $\frac{4!}{1!2!1!} p_a p_b^2 p_c$ , but this factor does not affect the maximization.)

(c) **Maximum likelihood estimators**

We maximize  $L$  subject to  $p_a + p_b + p_c = 1, p_i \geq 0$ .

Use the hint  $p_c = 1 - p_a - p_b$  and write

$$L(p_a, p_b) = p_a p_b^2 (1 - p_a - p_b),$$

for  $p_a \geq 0, p_b \geq 0, p_a + p_b \leq 1$ .

It is convenient to maximize the log-likelihood:

$$\ell(p_a, p_b) = \log L = \log p_a + 2 \log p_b + \log(1 - p_a - p_b),$$

for  $0 < p_a, p_b, p_a + p_b < 1$ .

Compute partial derivatives:

$$\frac{\partial \ell}{\partial p_a} = \frac{1}{p_a} - \frac{1}{1 - p_a - p_b}, \quad \frac{\partial \ell}{\partial p_b} = \frac{2}{p_b} - \frac{1}{1 - p_a - p_b}.$$



Set these to zero for an interior maximum:

$$\frac{1}{p_a} = \frac{1}{1 - p_a - p_b} \Rightarrow p_a = 1 - p_a - p_b \Rightarrow 2p_a + p_b = 1,$$

$$\frac{2}{p_b} = \frac{1}{1 - p_a - p_b} \Rightarrow 2(1 - p_a - p_b) = p_b \Rightarrow 2 - 2p_a - 2p_b = p_b \Rightarrow 2 - 2p_a = 3p_b.$$

From  $2p_a + p_b = 1$  we get  $p_b = 1 - 2p_a$ . Substitute into  $2 - 2p_a = 3p_b$ :

$$2 - 2p_a = 3(1 - 2p_a) = 3 - 6p_a \Rightarrow 2 - 2p_a = 3 - 6p_a \Rightarrow 4p_a = 1 \Rightarrow p_a = \frac{1}{4}.$$

Then

$$p_b = 1 - 2p_a = 1 - \frac{2}{4} = \frac{1}{2},$$

and

$$p_c = 1 - p_a - p_b = 1 - \frac{1}{4} - \frac{1}{2} = \frac{1}{4}.$$

Thus the MLEs are

$$\hat{p}_a = \frac{1}{4}, \quad \hat{p}_b = \frac{1}{2}, \quad \hat{p}_c = \frac{1}{4},$$

which coincide with the observed relative frequencies.